ascii_is_utf8

src/cbor/spec/raw/CBOR.Spec.API.UTF8.fst
@@ -1,2 +1,3 @@
 module CBOR.Spec.API.UTF8
 let correct = CBOR.Spec.Raw.Format.UTF8.correct
+let ascii_is_utf8 = CBOR.Spec.Raw.Format.UTF8.ascii_is_utf8
