src/cbor/spec/raw/CBOR.Spec.Raw.Format.UTF8.fsti
@@ -4,3 +4,9 @@ module U8 = FStar.UInt8
 // Correctness of UTF-8 strings
 noextract [@@noextract_to "krml"]
 val correct: (Seq.seq U8.t) -> bool
+
+val ascii_is_utf8
+  (s: Seq.seq U8.t)
+: Lemma
+  (requires (forall i . i < Seq.length s ==> U8.v (Seq.index s i) < 128))
+  (ensures (correct s))
